%===============================================================================
\section{Temporal Discretization}
%===============================================================================
\subsection{Fluid Momentum Source Update Equation}
%-------------------------------------------------------------------------------
\subsubsection{Crank-Nicolson}
%-------------------------------------------------------------------------------
For a step $t^n\rightarrow t^{n+1}$,
\begin{equation}
  \frac{\rho^{n+1}\left(u^{k+1}-u^*\right)}{\dt} = 
   \half\left[\frac{\sigma_{t}}{c}\left(\F-\frac{4}{3}\E u\right)\right]^n
  +\half\left[\frac{\sigma_{t}}{c}\left(\F-\frac{4}{3}\E u\right)\right]^k
  \pep
\end{equation}

\subsubsection{TR/BDF-2}
%-------------------------------------------------------------------------------
For a step $t^{n+\half}\rightarrow t^{n+1}$,
\begin{equation}\begin{split}
  \frac{\rho^{n+1}\left(u^{k+1}-u^*\right)}{\half\dt} =  
  & \sixth\left[\frac{\sigma_{t}}{c}\left(\F-\frac{4}{3}\E u\right)\right]^n
   +\sixth\left[\frac{\sigma_{t}}{c}\left(\F-\frac{4}{3}\E u\right)\right]^{n+\half}\\
  &+\frac{2}{3}\left[\frac{\sigma_{t}}{c}\left(\F-\frac{4}{3}\E u\right)\right]^{k+1}
  \pep
\end{split}\end{equation}

\subsection{Fluid Energy Source Update Equation}
%-------------------------------------------------------------------------------
\subsubsection{Crank-Nicolson}
%-------------------------------------------------------------------------------
For a step $t^n\rightarrow t^{n+1}$,
\begin{equation}\begin{split}
  \frac{E^{k+1}-E^*}{\dt} = &
  -\half\left[\sigma_{a} c\left(aT^4 - \E\right)\right]^n
  -\half\sigma_{a}^k c\left[aT^4 - \E\right]^{k+1}\\
  &+\half\left[\sigma_{t}\frac{u}{c}\left(\F-\frac{4}{3}\E u\right)\right]^n
   +\half\left[\sigma_t\frac{u}{c}\left(\F-\frac{4}{3}\E u\right)\right]^k
  \pep
\end{split}\end{equation}

\subsubsection{TR/BDF-2}
%-------------------------------------------------------------------------------
For a step $t^{n+\half}\rightarrow t^{n+1}$,
\begin{equation}\begin{split}
  \frac{E^{k+1}-E^*}{\half\dt} = &
  -\sixth\left[\sigma_a c\left(aT^4 - \E\right)\right]^n
  -\sixth\left[\sigma_a c\left(aT^4 - \E\right)\right]^{n+\half}\\
  &-\frac{2}{3}\sigma_a^k c\left[aT^4 - \E\right]^{k+1}
   +\sixth\left[\sigma_t\frac{u}{c}\left(\F-\frac{4}{3}\E u\right)\right]^n\\
  &+\sixth\left[\sigma_t\frac{u}{c}\left(\F-\frac{4}{3}\E u\right)\right]^{n+\half}
   +\frac{2}{3}\left[\sigma_t\frac{u}{c}\left(\F-\frac{4}{3}\E u\right)\right]^k
  \pep
\end{split}\end{equation}


\subsection{\texorpdfstring{S$_2$}{S-2} Equations}
%-------------------------------------------------------------------------------
\subsubsection{Crank-Nicolson}
%-------------------------------------------------------------------------------
Applying the Crank-Nicolson scheme to Equation \requ{S2Q} for a step
$t^n\rightarrow t^{n+1}$, the S-2 equations become
%\begin{equation}\lequ{S2CN}\begin{split}
%  \frac{1}{c}\frac{\psi^{\pm,k+1}-\psi^{\pm,n}}{\dt} = &
%  -\half\mu^\pm\dydx{\psi^{\pm,n}} -\half\mu^\pm\dydx{\psi^{\pm,k+1}}\\
%  &-\half\sigma_t^n\psi^{\pm,n} -\half\sigma_t^k\psi^{\pm,k+1}\\
%  &+\half\frac{\sigma_s^n}{4\pi}\phi^n +\half\frac{\sigma_s^k}{4\pi}\phi^{k+1}\\
%  &+\half\frac{1}{4\pi}Q^{\pm,n} +\half\frac{1}{4\pi}Q^{\pm,k} \pec
%\end{split}\end{equation}
\begin{equation}\lequ{S2CN}\begin{split}
  \frac{1}{c}\frac{\Psi^{\pm,k+1}-\Psi^{\pm,n}}{\dt} = &
  -\half\mu^\pm\dydx{\Psi^{\pm,n}} -\half\mu^\pm\dydx{\Psi^{\pm,k+1}}\\
  &-\half\sigma_t^n\Psi^{\pm,n} -\half\sigma_t^k\Psi^{\pm,k+1}\\
  &+\half\frac{\sigma_s^n}{2}\phi^n +\half\frac{\sigma_s^k}{2}\phi^{k+1}\\
  &+\half\Q^{\pm,n} +\half\Q^{\pm,k} \pec
\end{split}\end{equation}
where $k$ represents the $k$th iteration of a quantity at time $t^{n+1}$.

\subsubsection{TR/BDF-2}
%-------------------------------------------------------------------------------
Applying the BDF-2 scheme to Equation \requ{S2Q} for a step
$t^{n}\rightarrow t^{n+1}$, the S-2 equations become
%\begin{equation}\lequ{S2BDF2}\begin{split}
%  \frac{1}{c}\frac{\psi^{\pm,k+1}-\psi^{\pm,n}}{\dt} = &
%  -\sixth\mu^\pm\dydx{\psi^{\pm,n-1}}
%  -\sixth\mu^\pm\dydx{\psi^{\pm,n}}
%  -\frac{2}{3}\mu^\pm\dydx{\psi^{\pm,k+1}}\\
%  &-\sixth\sigma_t^{n-1}\psi^{\pm,n-1}
%   -\sixth\sigma_t^{n}  \psi^{\pm,n}
%   -\frac{2}{3}\sigma_t^k\psi^{\pm,k+1}\\
%  &+\sixth\frac{\sigma_s^{n-1}}{4\pi}\phi^{n-1}
%   +\sixth\frac{\sigma_s^{n}}{4\pi}  \phi^{n}
%   +\frac{2}{3}\frac{\sigma_s^k}{4\pi}\phi^{k+1}\\
%  &+\sixth\frac{1}{4\pi}Q^{\pm,n-1}
%   +\sixth\frac{1}{4\pi}Q^{\pm,n}
%   +\frac{2}{3}\frac{1}{4\pi}Q^{\pm,k} \pec
%\end{split}\end{equation}
\begin{equation}\lequ{S2BDF2}\begin{split}
  \frac{1}{c}\frac{\Psi^{\pm,k+1}-\Psi^{\pm,n}}{\dt} = &
  -\sixth\mu^\pm\dydx{\Psi^{\pm,n-1}}
  -\sixth\mu^\pm\dydx{\Psi^{\pm,n}}
  -\frac{2}{3}\mu^\pm\dydx{\Psi^{\pm,k+1}}\\
  &-\sixth\sigma_t^{n-1}\Psi^{\pm,n-1}
   -\sixth\sigma_t^{n}  \Psi^{\pm,n}
   -\frac{2}{3}\sigma_t^k\Psi^{\pm,k+1}\\
  &+\sixth\frac{\sigma_s^{n-1}}{2}\phi^{n-1}
   +\sixth\frac{\sigma_s^{n}}{2}  \phi^{n}
   +\frac{2}{3}\frac{\sigma_s^k}{2}\phi^{k+1}\\
  &+\sixth\Q^{\pm,n-1}
   +\sixth\Q^{\pm,n}
   +\frac{2}{3}\Q^{\pm,k} \pec
\end{split}\end{equation}
where $k$ represents the $k$th iteration of a quantity at time $t^{n+1}$.
